Evaluator for V in CompilImp instead of within functor.

src/vminus/OpSemEval.v
@@ -3,6 +3,10 @@
 Require Import String.
 Require Import Vminus.Vminus.
 
+Require Import Vminus.CompilImp.
+Import ListCFG.
+Import V.Opsem.
+
 (* Some monadic set-up *)
 
 Definition err (A : Type) : Type := (string + A)%type.
@@ -17,149 +21,135 @@ Definition err_ret {A : Type} (a : A) : err A :=
 
 Notation "'do' x <- y ; z" := (err_bind y (fun x => z)) (at level 90).
 
-Module MakeEval (Import Cfg:CFG).
+(** *** Small-step, executable operational semantics *)
 
-Module SS := Make Cfg. 
-Import SS.
-
-
-Module Evaluator.
-  (** *** Small-step, executable operational semantics *)
-
-  Fixpoint eval_step (g : Cfg.t) (s : state) : err state :=
-    let 'mkst mem pc loc ppc ploc := s in
-    match (fetch g pc) with
-    | Some (uid, cmd_bop bop v1 v2) =>    
-      let result := eval_bop loc bop v1 v2 in
-      match result with
-      | Some n => inr (mkst mem (incr_pc pc) (update loc uid (Some n)) ppc ploc)
-      | None => inl "cannot evalute binop command"%string
-      end 
-    | Some (uid, cmd_phi pas) =>
-      let result := eval_phi ploc (lbl_of ppc) pas in
-      match result with
-      | Some n => inr (mkst mem (incr_pc pc) (update loc uid (Some n)) ppc ploc)
-      | None => inl "cannot evaluate phi"%string
-      end
-    | Some (uid, cmd_tmn tmn) =>
-      let result := eval_tmn loc tmn in
-      match result with
-      | Some l' => inr (mkst mem (block_entry l') loc pc loc)
-      | None => inl "cannot evaluate terminator"%string
-      end
-    | Some (uid, cmd_load addr) =>
-      inr (mkst mem (incr_pc pc) (update loc uid (Some (mem addr))) ppc ploc)
-    | Some (uid, cmd_store addr v) => 
-      let result := eval_val loc v in
-      match result with
-      (* | Some n => BUG HERE
+Fixpoint eval_step (g : cfg) (s : state) : err state :=
+  let 'mkst mem pc loc ppc ploc := s in
+  match (fetch g pc) with
+  | Some (uid, cmd_bop bop v1 v2) =>    
+    let result := V.Opsem.eval_bop loc bop v1 v2 in
+    match result with
+    | Some n => inr (mkst mem (incr_pc pc) (update loc uid (Some n)) ppc ploc)
+    | None => inl "cannot evalute binop command"%string
+    end 
+  | Some (uid, cmd_phi pas) =>
+    let result := eval_phi ploc (lbl_of ppc) pas in
+    match result with
+    | Some n => inr (mkst mem (incr_pc pc) (update loc uid (Some n)) ppc ploc)
+    | None => inl "cannot evaluate phi"%string
+    end
+  | Some (uid, cmd_tmn tmn) =>
+    let result := eval_tmn loc tmn in
+    match result with
+    | Some l' => inr (mkst mem (block_entry l') loc pc loc)
+    | None => inl "cannot evaluate terminator"%string
+    end
+  | Some (uid, cmd_load addr) =>
+    inr (mkst mem (incr_pc pc) (update loc uid (Some (mem addr))) ppc ploc)
+  | Some (uid, cmd_store addr v) => 
+    let result := eval_val loc v in
+    match result with
+    (* | Some n => BUG HERE
            inr (mkst (Memory.update mem addr n) (incr_pc pc) loc pc ploc) *)
-      | Some n => inr (mkst (Memory.update mem addr n) (incr_pc pc) loc ppc ploc)
-      | None => inl "cannot evaluate address to store to"%string
-      end
-    | None => inl "no instruction fetched"%string
-    end.
+    | Some n => inr (mkst (Memory.update mem addr n) (incr_pc pc) loc ppc ploc)
+    | None => inl "cannot evaluate address to store to"%string
+    end
+  | None => inl "no instruction fetched"%string
+  end.
 
-  Fixpoint eval_until_pc (g : Cfg.t) (s : state)
-           (target_pc: pc)
-           (fuel : nat): err state :=
-    match fuel with
-    | 0 => inl "eval out of fuel"%string
-    | S n' =>
-      if (eq_dec_pc (st_pc s) target_pc) then inr s
-      else match eval_step g s with
-           | inl err => inl err
-           | inr s' => eval_until_pc g s' target_pc n'
-           end
-    end.
+Fixpoint eval_until_pc (g : cfg) (s : state)
+         (target_pc: pc)
+         (fuel : nat): err state :=
+  match fuel with
+  | 0 => inl "eval out of fuel"%string
+  | S n' =>
+    if (eq_dec_pc (st_pc s) target_pc) then inr s
+    else match eval_step g s with
+         | inl err => inl err
+         | inr s' => eval_until_pc g s' target_pc n'
+         end
+  end.
 
-End Evaluator.
 
-Module EvaluatorCorrect.
-  Import Evaluator.
+Ltac eval_step_with_step next_state constructor_rule
+     cfg_well_formed fetched :=
+  match goal with
+  | H: match ?X with
+       | Some _ => _
+       | None => _ end = inr ?next_state |-
+    step ?cfg ?curr_state next_state =>
+    destruct X eqn:Heval;
+    inversion H;
+    eapply constructor_rule;
+    try rewrite insn_at_pc_fetch;
+    try apply fetched;
+    try apply cfg_well_formed;
+    rewrite Heval;
+    reflexivity
+  | H : _ = inr next_state |-
+    step ?cfg ?curr_state next_state =>
+    inversion H;
+    eapply constructor_rule;
+    try rewrite insn_at_pc_fetch;
+    try apply fetched;
+    try apply cfg_well_formed;
+    reflexivity
+  end.
 
-  Ltac eval_step_with_step next_state constructor_rule
-       cfg_well_formed fetched :=
-    match goal with
-    | H: match ?X with
-         | Some _ => _
-         | None => _ end = inr next_state |-
-      step ?cfg ?curr_state next_state =>
-      
-      destruct X eqn:Heval; 
-      inversion H;
-      eapply constructor_rule;
-      try rewrite insn_at_pc_fetch;
-      try apply fetched;
-      try apply cfg_well_formed;
-      rewrite Heval;
-      reflexivity
-    | H : _ = inr next_state |-
-      step ?cfg ?curr_state next_state =>
-      
-      inversion H;
-      eapply constructor_rule;
-      try rewrite insn_at_pc_fetch;
-      try apply fetched;
-      try apply cfg_well_formed;
-      reflexivity
-    end.
+Ltac cases_on_eval_step_in_goal eval_insn :=
+  match goal with
+  | |- match ?X with
+      | Some _ => _
+      | None => _ end = inr _  =>
+    destruct X;
+    inversion eval_insn;
+    reflexivity
+  end.
 
-  Ltac cases_on_eval_step_in_goal eval_insn :=
-    match goal with
-    | |- match ?X with
-        | Some _ => _
-        | None => _ end = inr _  =>
-      destruct X;
-      inversion eval_insn;
-      reflexivity
-    end.
-
-  Lemma evaluator_sound: forall g s s',
-      wf_cfg g -> eval_step g s = inr s' -> step g s s'.
-  Proof.
-    intros g s s' wf_g.
+Lemma evaluator_sound: forall g s s',
+    wf_cfg g -> eval_step g s = inr s' -> step g s s'.
+Proof.
+  intros g s s' wf_g; unfold eval_step;
+    destruct g as [entry blks] eqn:g_eq;
+    rewrite <- g_eq in *;
     destruct s as [mem curr_pc curr_loc previous_pc previous_loc];
-      simpl.
     destruct (fetch g curr_pc) as 
         [[uid [bop v1 v2 | pas | term | addr | addr v]] | ] eqn:fetched;
-      intros H;
-      [eval_step_with_step s' step_bop wf_g fetched |
-       eval_step_with_step s' step_phi wf_g fetched |
-       eval_step_with_step s' step_tmn wf_g fetched |
-       eval_step_with_step s' step_load wf_g fetched |
-       eval_step_with_step s' step_store wf_g fetched | idtac].
-    inversion H.
-  Qed.
-    
-  Lemma evaluator_complete: forall g s s',
-      wf_cfg g -> step g s s' -> eval_step g s = inr s'.
-  Proof.
-    intros g s s' wf_g step_rel.
-    inversion step_rel as
-        [mem pc loc bop v1 v2 uid n ppc ploc insn_at_pc_is eval_insn_ok s_eq s'_eq |
-         mem pc loc pas uid n ppc ploc insn_at_pc_is eval_insn_ok s_eq s'_eq |
-         mem pc label loc term uid ppc ploc insn_at_pc_is eval_insn_ok s_eq s'_eq |
-         mem pc loc uid addr ppc ploc insn_at_pc_is eval_insn_ok s'_eq |
-         mem pc loc uid addr v n ppc ploc insn_at_pc_is eval_insn_ok s_eq s'_eq];
-      simpl;
-      destruct (fetch g pc) as [[curr_uid curr_cmd] | ] eqn:fetched; 
-      rewrite insn_at_pc_fetch in insn_at_pc_is; try apply wf_g;
-        rewrite insn_at_pc_is in fetched;
-        inversion fetched;
-        try cases_on_eval_step_in_goal eval_insn_ok.
-    reflexivity.
-  Qed.
+    intros H;
+    [eval_step_with_step s' step_bop wf_g fetched |
+     eval_step_with_step s' step_phi wf_g fetched |
+     eval_step_with_step s' step_tmn wf_g fetched |
+     eval_step_with_step s' step_load wf_g fetched |
+     eval_step_with_step s' step_store wf_g fetched | idtac].
+  inversion H.
+Qed.
 
-  Theorem evaluator_correct: forall g s s',
-      wf_cfg g -> eval_step g s = inr s' <-> step g s s'.
-  Proof.
-    intros g s s' wf_g; split;
-      revert g s s' wf_g.
-    apply evaluator_sound.
-    apply evaluator_complete.
-  Qed.
+Lemma evaluator_complete: forall g s s',
+    wf_cfg g -> step g s s' -> eval_step g s = inr s'.
+Proof.
+  intros g s s' wf_g step_rel; unfold eval_step;
+    destruct g as [entry blks] eqn:g_eq;
+    rewrite <- g_eq in *.
+  inversion step_rel as
+      [mem pc loc bop v1 v2 uid n ppc ploc insn_at_pc_is eval_insn_ok s_eq s'_eq |
+       mem pc loc pas uid n ppc ploc insn_at_pc_is eval_insn_ok s_eq s'_eq |
+       mem pc label loc term uid ppc ploc insn_at_pc_is eval_insn_ok s_eq s'_eq |
+       mem pc loc uid addr ppc ploc insn_at_pc_is eval_insn_ok s'_eq |
+       mem pc loc uid addr v n ppc ploc insn_at_pc_is eval_insn_ok s_eq s'_eq];
+    simpl;
+    destruct (fetch g pc) as [[curr_uid curr_cmd] | ] eqn:fetched; 
+    rewrite insn_at_pc_fetch in insn_at_pc_is; try apply wf_g;
+      rewrite insn_at_pc_is in fetched;
+      inversion fetched;
+      try cases_on_eval_step_in_goal eval_insn_ok.
+  reflexivity.
+Qed.
 
-End EvaluatorCorrect.
-    
-End MakeEval.
+Theorem evaluator_correct: forall g s s',
+    wf_cfg g -> eval_step g s = inr s' <-> step g s s'.
+Proof.
+  intros g s s' wf_g; split;
+    revert g s s' wf_g.
+  apply evaluator_sound.
+  apply evaluator_complete.
+Qed.
